
\documentclass[11pt, oneside]{article}   	

\usepackage{color}
\usepackage{graphicx}				
\usepackage{prfblock}
\usepackage{amssymb}
\newtheorem{Theorem}{Theorem}
\newtheorem{Lemma}{Lemma}
\newtheorem{Proposition}{Proposition}
\newtheorem{Definition}{Definition}
\newtheorem{Axiom}{Axiom}
 \usepackage{tcolorbox}
 \tcbuselibrary{skins}
 \tcbuselibrary{theorems}
\tcbuselibrary{breakable}


\newcommand{\mybox}[1]{\begin{tcolorbox}[colback=white,colframe=gray!20!white, breakable, skin=enhancedmiddle]#1 \end{tcolorbox}}
\title{Brief Article}
\author{The Author}
\date{}							% Activate to display a given date or no date

\begin{document}
\maketitle

\begin{Definition}[divides] 
$divides\,(a\,b:nat)\,:=\,âˆƒ\,x:nat,\,b\,=\,a*x.
$
 \end{Definition}
\begin{Theorem}[refldiv] 
$\forall \,a\,b\,c,\,(a\,|\,b)\,\land (b\,|\,c)\,\Rightarrow \,(a\,|c).$
 \end{Theorem}


 Proof: \begin{subproof}In order to show $\forall a b c : nat, a | b \land b | c \Rightarrow a | c $ we pick an arbitrary $a$ and show $\forall b c : nat, a | b \land b | c \Rightarrow a | c $.

 \begin{subproof}In order to show $\forall b c : nat, a | b \land b | c \Rightarrow a | c $ we pick an arbitrary $b$ and show $\forall c : nat, a | b \land b | c \Rightarrow a | c $.

 \begin{subproof}In order to show $\forall c : nat, a | b \land b | c \Rightarrow a | c $ we pick an arbitrary $c$ and show $a | b \land b | c \Rightarrow a | c $.

 \begin{subproof}We will assume $Hyp : a | b \land b | c $ and show $a | c $.\begin{subproof}Since we know $Hyp : a | b \land b | c $ we also know $Hyp0 : a | b 
Hyp1 : b | c $.\begin{subproof}We use the definition of $divides$ in $Hyp0$ to obtain $Hyp0 : \exists x : nat, b = a * x $ \begin{subproof}We use the definition of $divides$ in $Hyp1$ to obtain $Hyp1 : \exists x : nat, c = b * x $ \begin{subproof}Rewriting the definition of $divides$ in our conclusion $a | c $, we now need to show $\exists x : nat, c = a * x $.\begin{subproof}We choose a variable $x$ in $Hyp1$ to obtain $x : nat 
Hyp1 : c = b * x $.\begin{subproof}We rewrite the goal using $Hyp1$ to obtain $\exists x0 : nat, b * x = a * x0 $.\begin{subproof}We choose a variable $y$ in $Hyp0$ to obtain $a, b, c, y : nat 
Hyp0 : b = a * y $.\begin{subproof}We rewrite the goal using $Hyp0$ to obtain $\exists x0 : nat, a * y * x = a * x0 $.\begin{subproof}We shall prove $\exists x0 : nat, a * y * x = a * x0 $ by showing $a * y * x = a * (y * x) $.\begin{subproof}This follows immediately from arithmetic.\begin{subproof}This is done\end{subproof}\end{subproof} Now $a * y * x = a * (y * x) $ means that $\exists x0 : nat, a * y * x = a * x0 $.\end{subproof} We have now proved $\exists x0 : nat, a * y * x = a * x0 $ and so $\exists x0 : nat, b * x = a * x0 $ follows.\end{subproof} and so we have proved $\exists x0 : nat, b * x = a * x0 $.\end{subproof} We have now proved $\exists x0 : nat, b * x = a * x0 $ and so $\exists x0 : nat, c = a * x0 $ follows.\end{subproof} and so we have proved $\exists x : nat, c = a * x $.\end{subproof} Therefore we have showed $\exists x : nat, c = a * x $ and so $a | c $.\end{subproof} therefore we have $a | c $.\end{subproof} therefore we have $a | c $.\end{subproof} We are now done with $a | c $.\end{subproof} We have now showed that if $Hyp : a | b \land b | c $ then $a | c $ a proof of $a | b \land b | c \Rightarrow a | c $.\end{subproof} Since $c$ was arbitrary this shows $\forall c : nat, a | b \land b | c \Rightarrow a | c $.\end{subproof} Since $b$ was arbitrary this shows $\forall b c : nat, a | b \land b | c \Rightarrow a | c $.\end{subproof} Since $a$ was arbitrary this shows $\forall a b c : nat, a | b \land b | c \Rightarrow a | c $.\end{subproof}This is done\end{document}
