\part{ Description of the tactics and hints}
\chapter{Tactics}

\section{This is trivial.}

This will only work on very easy statements. If it works it will solve the current goal. Try to avoid overuse. Do better than your lecturers.


\section{I cannot prove this.}

If you are stuck this tactic will ``prove'' the current goal. If you use this in a proof at the end if the proof when you try to use Qed you will get the following error
\mess{``Error:Attempt to save a proof with given up goals. If this is really what
you want to do, use Admitted in place of Qed.}
To avoid the error just type Admitted instead of Qed.


\section{Prove left hand side.}
Suppose you want to prove the following goal:
\coq{\cdots\\ 
===== \\ 
P\lor Q}

The above mentioned tactic will the produce a the following goal

\coq{\cdots\\ 
===== \\ 
P}
 and so you will have to now prove a simple goal.

\section{Prove right hand side.}
Symmetric with the above, suppose you want to prove the following goal:
\coq{\cdots\\ 
===== \\ 
P\lor Q}

The above mentioned tactic will the produce a the following goal

\coq{\cdots\\ 
===== \\ 
Q}



\section{Prove VAR in the disjunction.}
This tactic combines the above two. More precisely,
suppose you want to prove the following goal:
\coq{\cdots\\ 
===== \\ 
P\lor Q}

Then applying 
\inp{Prove P in the disjunction.}

will produce the goal 
\coq{\cdots\\ 
===== \\ 
P}
while applying
\inp{Prove Q in the disjunction.}

will produce the goal 
\coq{\cdots\\ 
===== \\ 
Q}

\section{Eliminate the conjuction in hypothesis VAR.}

Suppose your goal looks like
\coq{\cdots\\ 
Hyp: P\land Q\\
\cdots \\
===== \\ 
\cdots}

Then applying 
\inp{Eliminate the conjunction in hypothesis Hyp.}
will produce a goal similar to the one below:

\coq{\cdots\\ 
Hyp: P\\
Hyp0: Q\\
\cdots\\
===== \\ 
\cdots}
allowing you to use the parts of Hyp independently.


\section{Consider cases based on disjunction in hypothesis VAR.}
Suppose your goal looks like
\coq{\cdots\\ 
Hyp: P\lor Q\\
\cdots \\
===== \\ 
\cdots}
Then applying 
\inp{Consider cases based on disjunction in hypothesis Hyp.}
will produce two separate goals similar to the one below:
\coq{\cdots\\ 
Hyp: P\\
\cdots \\
===== \\ 
\cdots}

\coq{\cdots\\ 
Hyp: Q\\
\cdots \\
===== \\ 
\cdots}

obtaining a proof by cases.

\section{Prove the conjunction in the goal by first proving VAR then VAR.}
Suppose your goal looks like
\coq{\cdots\\ 
===== \\ 
P\land Q}
 Then 
 \inp{Prove the conjunction in the goal by first proving P then Q.}
 
 will separate the proof in two different goals
 
 \coq{\cdots\\ 
===== \\ 
P}
\coq{\cdots\\ 
===== \\ 
Q}

 
\section{Assume VAR then prove VAR.}
Suppose your goal looks like
\coq{\cdots\\ 
===== \\ 
P\rightarrow Q}

then 
\inp{Assume P then prove Q.}
will modify the goal to

\coq{\cdots\\ 
P\\
===== \\ 
Q}



\section{Prove both directions of VAR iff VAR.}

Suppose your goal looks like
\coq{\cdots\\ 
===== \\ 
P\leftrightarrow Q}

then 
\inp{Prove both directions of P iff Q.}
will split the goal into two different goals

\coq{\cdots\\ 
===== \\ 
P\rightarrow Q}

\coq{\cdots\\ 
===== \\ 
Q\rightarrow P}



\section{Fix an arbitrary element VAR.}

Suppose your goal looks like
\coq{\cdots\\ 
===== \\ 
\forall x:S, P(x) }

then 
\inp{Fix an arbitrary element a.}
will modify the goal to

\coq{\cdots\\ 
a:S\\
===== \\ 
P(a)}

\section{Fix VAR the existentially quantified variable in VAR.}
Suppose your goal looks like
\coq{\cdots\\ 
Hyp:\exists x:S, P(x)\\
===== \\ 
\cdots }

then 
\inp{Fix a the existentially quantified variable in Hyp.}
will modify the goal to

\coq{\cdots\\ 
a:S\\
Hyp:P(a)\\
===== \\ 
\cdots}


\section{Obtain VAR using variable VAR in the universally quantified hypothesis VAR.}
Suppose your goal looks like
\coq{\cdots\\ 
Hyp:\forall x:S, P(x)\\
===== \\ 
\cdots }

then 

\inp{Obtain Q using variable a in the universally quantified hypothesis Hyp.}

will attempt to apply the result $P(a)$ to prove the result $Q$.

\section{Prove the existential claim is true for VAR.}

Suppose your goal looks like
\coq{\cdots\\ 
===== \\ 
\exists x:S, P(x) }

then 
\inp{Prove the existential claim is true for a.}
will modify the goal to

\coq{\cdots\\ 
===== \\ 
P(a)}


\inp{Rewrite the goal using VAR.}

Suppose your goal looks like
\coq{\cdots\\ 
Hyp: x= f\\
===== \\ 
 P(x) }

then 
\inp{Rewrite the goal using Hyp.}
will replace every occurrence of x in P by f. Similarly if the goal is 

\coq{\cdots\\ 
Hyp: x= f\\
===== \\ 
 P(f) }

\inp{Rewrite the goal using Hyp.}
will replace every occurrence of f in P by x.  

Finally if Thm is a theorem whose conclusion includes and equality $x=f$ and if the goal of your theorem looks like

\coq{\cdots\\ 
===== \\ 
 P(x) }
 Then 
\inp{Rewrite the goal using Thm.}
will replace every occurrence of x in P by f.  



\section{True by arithmetic properties.}

This tactic will attempt to prove the statement by using the ring properties (commutativity, associativity and distributivity) of the natural, integers or reals. 

\section{Claim VAR by rewriting VAR using VAR.}

This is very similar to \inp{Rewrite the goal using VAR.}

The idea is that 
\inp{Claim Q by rewriting Hyp using Thm.}

Will attempt to prove the statement $Q$ by applying the rewritten version of $Hyp$. the rules for $Thm$ are as above.

\section{Claim VAR.}

This is forward proof tactic. 
\inp{Claim P.}

will introduce a new claim, splitting the goal

\coq{\cdots\\ 
===== \\ 
Q }

into 

\coq{\cdots\\ 
===== \\ 
 P }
and 

\coq{\cdots\\ 
Hyp:P\\
===== \\ 
 Q }





\section{Rewrite hypothesis VAR using the definition of VAR.}
If the hypothesis Hyp will involve a previous definition d, then
\inp{Rewrite hypothesis Hyp using the definition of d.}
 will unfold a definition of d inside Hyp.

\section{Apply induction on VAR.}

This is a rather general tactic. It will generally act as an induction omnibus. More precisely

\inp{Apply induction on n.}
will depend on the (inductive) type of n. For example if $n$ is a natural number and the goal is

\coq{\cdots\\ 
===== \\ 
 P(n) }
 then 
\inp{Apply induction on n.}

will split the proof into two goals
\coq{\cdots\\ 
===== \\ 
 P(0) }
 
 and 
 
 \coq{\cdots\\ 
 IHn:P(n)\\
===== \\ 
 P( S n) }
On the other hand if $n$ is an integer, the goal
\coq{\cdots\\ 
===== \\ 
 P(n) }
will be split into 3 cases

\coq{\cdots\\ 
===== \\ 
 P(0) }
 
 \coq{\cdots\\ 
 n:positive
===== \\ 
 P(Z.pos\  n) }
 
  \coq{\cdots\\ 
 n:negative
===== \\ 
 P(Z.neg\  n) }

\section{Rewrite goal using the definition of VAR.}
If the goal will involve a previous definition d, then
\inp{Rewrite goal using the definition of d.}
 will unfold a definition of d inside the conclusion of the goal.


\section{obtain VAR applying VAR to VAR}.

\section{Prove by contradiction.}

Assume the goal is:

\coq{\cdots\\ 
===== \\ 
 P }
 
 then  
 \inp{Prove by contradiction.} will transform the goal to
 
 \coq{\cdots\\ 
 \not P\\
===== \\ 
 False}


This follows from reflexivity.


This follows from symmetry.


Apply result VAR.


This follows from assumptions.

Denote VAR by VAR.